theories/simplang/primitive_laws.v
@@ -526,15 +526,15 @@ Proof.
 Qed.
 
 (** Call lemmas for sim *)
-Lemma sim_call π e_t e_s v_t v_s f :
+Lemma sim_call π e_t e_s v_t v_s fname :
   to_val e_t = Some v_t →
   to_val e_s = Some v_s →
-  ⊢ ext_rel π v_t v_s -∗ Call (## f) e_t ⪯{π} Call (## f) e_s {{ ext_rel π }}.
+  ⊢ ext_rel π v_t v_s -∗ Call (f#fname) e_t ⪯{π} Call (f#fname) e_s {{ ext_rel π }}.
 Proof.
   intros <-%of_to_val <-%of_to_val.
   (* FIXME use lifting lemma for this *)
   iIntros "H". rewrite /sim /sim_stutter /sim_def sim_expr_unfold. iIntros (??????) "[(?&?&?&?&Hinv) [% %]]". iModIntro.
-  iRight; iRight. iExists f, empty_ectx, v_t, empty_ectx, v_s, σ_s.
+  iRight; iRight. iExists fname, empty_ectx, v_t, empty_ectx, v_s, σ_s.
   rewrite list_insert_id /= //. iFrame.
   iSplitR; first done. iSplitR. { iPureIntro. constructor. }
   iIntros (v_t' v_s' ) "H". iApply sim_value. iApply "H".
@@ -590,10 +590,10 @@ Lemma sim_while_rec b_t c_t v_s (K_s : ectx) (inv : val → iProp Σ) Ψ rec_n �
   rec_n @s K_s -∗
   □ (∀ v_s', inv v_s' -∗
     (if: c_t then b_t ;; while: c_t do b_t od else #())%E ⪯{π} (fill K_s v_s')%E
-    [{ λ e_t e_s , Ψ e_t e_s ∨ (∃ v_s', ⌜e_t = while: c_t do b_t od%E⌝ ∗ ⌜e_s = Call ##rec_n (Val v_s')⌝ ∗ inv v_s') }]) -∗
-  (while: c_t do b_t od ⪯{π} Call ## rec_n v_s [{ Ψ }])%E.
+    [{ λ e_t e_s , Ψ e_t e_s ∨ (∃ v_s', ⌜e_t = while: c_t do b_t od%E⌝ ∗ ⌜e_s = Call f#rec_n (Val v_s')⌝ ∗ inv v_s') }]) -∗
+  (while: c_t do b_t od ⪯{π} Call f#rec_n v_s [{ Ψ }])%E.
 Proof.
-  iIntros "Hinv #Hrec #Hstep". iApply (sim_lift_head_coind (λ e_t e_s, (∃ v_s', ⌜e_t = while: c_t do b_t od%E⌝ ∗ ⌜e_s = Call ##rec_n (Val v_s')⌝ ∗ inv v_s')%I)); first last.
+  iIntros "Hinv #Hrec #Hstep". iApply (sim_lift_head_coind (λ e_t e_s, (∃ v_s', ⌜e_t = while: c_t do b_t od%E⌝ ∗ ⌜e_s = Call f#rec_n (Val v_s')⌝ ∗ inv v_s')%I)); first last.
   { iExists v_s. eauto. }
   iModIntro. iIntros (?? ?? ?? ??) "He ((?&HP_s&?&?&?) & [% %])". iDestruct "He" as (v_s') "(-> & -> & Hinv)".
   iSpecialize ("Hstep" with "Hinv").
@@ -613,10 +613,10 @@ Lemma sim_rec_while b_s c_s v_t (K_t : ectx) (inv : val → iProp Σ) Ψ rec_n �
   rec_n @t K_t -∗
   □ (∀ v_t', inv v_t' -∗
     (fill K_t v_t')%E ⪯{π}  (if: c_s then b_s ;; while: c_s do b_s od else #())%E
-    [{ λ e_t e_s , Ψ e_t e_s ∨ (∃ v_t', ⌜e_t = Call ##rec_n (Val v_t')⌝ ∗ ⌜e_s = while: c_s do b_s od%E⌝ ∗  inv v_t') }]) -∗
-  ( Call ##rec_n v_t ⪯{π} while: c_s do b_s od [{ Ψ }])%E.
+    [{ λ e_t e_s , Ψ e_t e_s ∨ (∃ v_t', ⌜e_t = Call f#rec_n (Val v_t')⌝ ∗ ⌜e_s = while: c_s do b_s od%E⌝ ∗  inv v_t') }]) -∗
+  ( Call f#rec_n v_t ⪯{π} while: c_s do b_s od [{ Ψ }])%E.
 Proof.
-  iIntros "Hinv #Hrec #Hstep". iApply (sim_lift_head_coind (λ e_t e_s, (∃ v_t', ⌜e_t = Call ##rec_n (Val v_t')⌝ ∗ ⌜e_s = while: c_s do b_s od%E⌝ ∗  inv v_t'))%I); first last.
+  iIntros "Hinv #Hrec #Hstep". iApply (sim_lift_head_coind (λ e_t e_s, (∃ v_t', ⌜e_t = Call f#rec_n (Val v_t')⌝ ∗ ⌜e_s = while: c_s do b_s od%E⌝ ∗  inv v_t'))%I); first last.
   { iExists v_t. eauto. }
   iModIntro. iIntros (?? ?? ?? ??) "He ((HP_t & ? & ? & ? &?) & [% %])". iDestruct "He" as (v_s') "(-> & -> & Hinv)".
   iSpecialize ("Hstep" with "Hinv").
@@ -639,11 +639,11 @@ Lemma sim_rec_rec v_t v_s (K_t K_s : ectx) (inv : val → val → iProp Σ) Ψ r
   rec_s @s K_s -∗
   □ (∀ v_t' v_s', inv v_t' v_s' -∗
     (fill K_t v_t')%E ⪯{π} (fill K_s v_s')%E
-    [{ λ e_t e_s , Ψ e_t e_s ∨ (∃ v_t' v_s', ⌜e_t = Call ##rec_t (Val v_t')⌝ ∗ ⌜e_s = Call ##rec_s (Val v_s')⌝ ∗ inv v_t' v_s') }]) -∗
-  ( Call ##rec_t v_t ⪯{π} Call ##rec_s v_s [{ Ψ }])%E.
+    [{ λ e_t e_s , Ψ e_t e_s ∨ (∃ v_t' v_s', ⌜e_t = Call f#rec_t (Val v_t')⌝ ∗ ⌜e_s = Call f#rec_s (Val v_s')⌝ ∗ inv v_t' v_s') }]) -∗
+  ( Call f#rec_t v_t ⪯{π} Call f#rec_s v_s [{ Ψ }])%E.
 Proof.
   iIntros "Hinv #Hrec_t #Hrec_s #Hstep".
-  iApply (sim_lift_head_coind (λ e_t e_s, (∃ v_t' v_s', ⌜e_t = Call ##rec_t (Val v_t')⌝ ∗ ⌜e_s = Call ##rec_s (Val v_s')⌝ ∗ inv v_t' v_s'))%I); first last.
+  iApply (sim_lift_head_coind (λ e_t e_s, (∃ v_t' v_s', ⌜e_t = Call f#rec_t (Val v_t')⌝ ∗ ⌜e_s = Call f#rec_s (Val v_s')⌝ ∗ inv v_t' v_s'))%I); first last.
   { iExists v_t, v_s. eauto. }
   iModIntro. iIntros (?? ?? ?? ??) "He ((HP_t & HP_s & ? & ? &?) & [% %])".
   iDestruct "He" as (v_t' v_s') "(-> & -> & Hinv)".
@@ -654,7 +654,7 @@ Proof.
   iModIntro. iSplitR; first by eauto with head_step.
   iIntros (e_t' efs σ_t') "%Hhead"; inv_head_step.
   iModIntro.
-  assert (∃ e_s' σ_s', head_step P_s (Call ##rec_s v_s') σ_s e_s' σ_s' []) as (e_s' & σ_s' & Hred).
+  assert (∃ e_s' σ_s', head_step P_s (Call f#rec_s v_s') σ_s e_s' σ_s' []) as (e_s' & σ_s' & Hred).
   { eauto with head_step. }
   iExists e_s', σ_s'. inv_head_step. iFrame.
   iSplitR; [done|].
